Implement StateT

theories/Classes/Trans.v
@@ -5,8 +5,10 @@ Implicit Types t : (Type -> Type) -> (Type -> Type).
 Implicit Types m n : Type -> Type.
 
 Class MonadTrans t : Type :=
-  { lift : forall m a, m a -> t m a
+  { lift : forall m (Monad_m : Monad m) a, m a -> t m a
   }.
+
+Arguments lift {t _ m Monad_m} [a].
 
 Class MonadMorphism m n `{Monad m} `{Monad n} (f : forall a, m a -> n a) : Prop :=
   { morphism_pure : forall a (x : a), f _ (pure x) = pure x
@@ -14,4 +16,4 @@ Class MonadMorphism m n `{Monad m} `{Monad n} (f : forall a, m a -> n a) : Prop 
       f _ (bind u k) = bind (f _ u) (fun x => f _ (k x))
   }.
 
-Notation LawfulMonadTrans t := (forall m, MonadMorphism m (t m) lift).
+Notation LawfulMonadTrans t := (forall m `{LawfulMonad m}, MonadMorphism m (t m) lift).
