theories/Monads/Identity.v
@@ -1,0 +1,12 @@
+From mtl.Classes Require Import Monad.
+
+Record Identity (a : Type) : Type :=
+  MkIdentity { runIdentity : a }.
+
+Arguments MkIdentity {a} _.
+Arguments runIdentity {a} _.
+
+Instance Monad_Identity : Monad Identity :=
+  { pure _ := MkIdentity
+  ; bind _ _ u k := k (runIdentity u)
+  }.
