theories/Monads/State.v
@@ -1,0 +1,62 @@
+From Coq Require Import FunctionalExtensionality.
+
+From mtl.Classes Require Import Monad Trans State.
+From mtl.Monads Require Import Identity.
+
+Implicit Types s : Type.
+Implicit Types m n : Type -> Type.
+
+Record StateT s m (a : Type) : Type :=
+  MkStateT { runStateT : s -> m (a * s)%type }.
+
+Arguments MkStateT {s m a} _.
+Arguments runStateT {s m a} _.
+
+Instance Monad_StateT s m `{Monad m} : Monad (StateT s m) :=
+  { pure _ x := MkStateT (fun z => pure (x, z))
+  ; bind _ _ u k := MkStateT (fun z =>
+    runStateT u z >>= fun '(x, z1) =>
+    runStateT (k x) z1)
+  }.
+
+Instance MonadTrans_StateT s : MonadTrans (StateT s) :=
+  { lift _ _ _ u := MkStateT (fun z => u >>= fun x => pure (x, z))
+  }.
+
+Instance MonadState_StateT s m `{Monad m} : MonadState s (StateT s m) :=
+  { get := MkStateT (fun z => pure (z, z))
+  ; put z := MkStateT (fun _ => pure (tt, z))
+  }.
+
+Definition State s : Type -> Type := StateT s Identity.
+
+Lemma injective_runStateT s m a (u v : StateT s m a) :
+  runStateT u = runStateT v -> u = v.
+Proof.
+  destruct u, v; intros; f_equal; auto.
+Qed.
+
+Instance LawfulMonad_StateT s m `{LawfulMonad m} : LawfulMonad (StateT s m) := {}.
+Proof.
+  all: intros; apply injective_runStateT, functional_extensionality; intros; cbn.
+  - rewrite bind_pure_l. reflexivity.
+  - replace (fun _ => _) with (fun z : a * s => pure z).
+    2: apply functional_extensionality; intros []; auto.
+    rewrite bind_pure_r. reflexivity.
+  - rewrite bind_assoc.
+    f_equal. apply functional_extensionality. intros []. reflexivity.
+Qed.
+
+Instance LawfulMonadTrans_StateT s m : LawfulMonadTrans (StateT s) := {}.
+Proof.
+  all: intros; cbn; f_equal; apply functional_extensionality; intros.
+  - rewrite bind_pure_l; reflexivity.
+  - rewrite 2 bind_assoc; f_equal; apply functional_extensionality; intros.
+    rewrite bind_pure_l. reflexivity.
+Qed.
+
+Instance LawfulMonadState_StateT s m `{LawfulMonad m} : LawfulMonadState s (StateT s m) := {}.
+Proof.
+  all: intros; cbn; apply injective_runStateT, functional_extensionality; cbn; intros.
+  all: rewrite ?bind_pure_l; try reflexivity.
+Qed.
